Dependency/Test/regression/TestEx3/source.bpl
@@ -377,6 +377,7 @@ var {:extern} detChoiceCnt: int;
 function {:extern} DetChoiceFunc(a: int) : int;
 
 procedure {:extern} det_choice() returns (x: int);
+  modifies detChoiceCnt;
   ensures detChoiceCnt == INT_ADD(old(detChoiceCnt), 1);
   ensures x == DetChoiceFunc(old(detChoiceCnt));
 
@@ -488,51 +489,45 @@ axiom (forall M: [name][int]int, x: int, y: int :: { Unified(M[Field(x) := M[Fie
 
 function {:extern} value_is(c: int, e: int) : bool;
 
-const {:extern} {:model_const "e"} {:sourceFile "TestEx3.c"} {:sourceLine 16} unique __ctobpl_const_11: int;
+const {:extern} {:model_const "e"} {:sourceFile ".\source\testex3.c"} {:sourceLine 10} unique __ctobpl_const_1: int;
 
-const {:extern} {:model_const "e->op1"} {:sourceFile "TestEx3.c"} {:sourceLine 16} unique __ctobpl_const_10: int;
+const {:extern} {:model_const "e->oper"} {:sourceFile ".\source\testex3.c"} {:sourceLine 14} unique __ctobpl_const_4: int;
 
-const {:extern} {:model_const "e->op2"} {:sourceFile "TestEx3.c"} {:sourceLine 16} unique __ctobpl_const_12: int;
+const {:extern} {:model_const "e"} {:sourceFile ".\source\testex3.c"} {:sourceLine 20} unique __ctobpl_const_5: int;
 
-const {:extern} {:model_const "e"} {:sourceFile "TestEx3.c"} {:sourceLine 12} unique __ctobpl_const_13: int;
+const {:extern} {:model_const "e->result"} {:sourceFile ".\source\testex3.c"} {:sourceLine 20} unique __ctobpl_const_6: int;
 
-const {:extern} {:model_const "e"} {:sourceFile "TestEx3.c"} {:sourceLine 10} unique __ctobpl_const_1: int;
+const {:extern} {:model_const "e->oper"} {:sourceFile ".\source\testex3.c"} {:sourceLine 10} unique __ctobpl_const_2: int;
 
-const {:extern} {:model_const "e->result"} {:sourceFile "TestEx3.c"} {:sourceLine 20} unique __ctobpl_const_6: int;
+const {:extern} {:model_const "e"} {:sourceFile ".\source\testex3.c"} {:sourceLine 14} unique __ctobpl_const_3: int;
 
-const {:extern} {:model_const "e"} {:sourceFile "TestEx3.c"} {:sourceLine 16} unique __ctobpl_const_7: int;
+const {:extern} {:model_const "e->op2"} {:sourceFile ".\source\testex3.c"} {:sourceLine 16} unique __ctobpl_const_12: int;
 
-const {:extern} {:model_const "e->result"} {:sourceFile "TestEx3.c"} {:sourceLine 16} unique __ctobpl_const_8: int;
+const {:extern} {:model_const "e"} {:sourceFile ".\source\testex3.c"} {:sourceLine 12} unique __ctobpl_const_13: int;
 
-const {:extern} {:model_const "e"} {:sourceFile "TestEx3.c"} {:sourceLine 16} unique __ctobpl_const_9: int;
+const {:extern} {:model_const "e->op1"} {:sourceFile ".\source\testex3.c"} {:sourceLine 12} unique __ctobpl_const_16: int;
 
-const {:extern} {:model_const "e"} {:sourceFile "TestEx3.c"} {:sourceLine 14} unique __ctobpl_const_3: int;
+const {:extern} {:model_const "e"} {:sourceFile ".\source\testex3.c"} {:sourceLine 12} unique __ctobpl_const_15: int;
 
-const {:extern} {:model_const "e->oper"} {:sourceFile "TestEx3.c"} {:sourceLine 14} unique __ctobpl_const_4: int;
+const {:extern} {:model_const "e->op2"} {:sourceFile ".\source\testex3.c"} {:sourceLine 12} unique __ctobpl_const_18: int;
 
-const {:extern} {:model_const "e"} {:sourceFile "TestEx3.c"} {:sourceLine 20} unique __ctobpl_const_5: int;
+const {:extern} {:model_const "e->result"} {:sourceFile ".\source\testex3.c"} {:sourceLine 12} unique __ctobpl_const_14: int;
 
-const {:extern} {:model_const "e->oper"} {:sourceFile "TestEx3.c"} {:sourceLine 10} unique __ctobpl_const_2: int;
+const {:extern} {:model_const "e"} {:sourceFile ".\source\testex3.c"} {:sourceLine 12} unique __ctobpl_const_17: int;
 
-const {:extern} {:model_const "e->op2"} {:sourceFile "TestEx3.c"} {:sourceLine 12} unique __ctobpl_const_18: int;
+const {:extern} {:model_const "e"} {:sourceFile ".\source\testex3.c"} {:sourceLine 16} unique __ctobpl_const_7: int;
 
-const {:extern} {:model_const "e->result"} {:sourceFile "TestEx3.c"} {:sourceLine 12} unique __ctobpl_const_14: int;
+const {:extern} {:model_const "e->result"} {:sourceFile ".\source\testex3.c"} {:sourceLine 16} unique __ctobpl_const_8: int;
 
-const {:extern} {:model_const "e"} {:sourceFile "TestEx3.c"} {:sourceLine 12} unique __ctobpl_const_17: int;
+const {:extern} {:model_const "e"} {:sourceFile ".\source\testex3.c"} {:sourceLine 16} unique __ctobpl_const_9: int;
 
-const {:extern} {:model_const "e"} {:sourceFile "TestEx3.c"} {:sourceLine 12} unique __ctobpl_const_15: int;
+const {:extern} {:model_const "e"} {:sourceFile ".\source\testex3.c"} {:sourceLine 16} unique __ctobpl_const_11: int;
 
-const {:extern} {:model_const "e->op1"} {:sourceFile "TestEx3.c"} {:sourceLine 12} unique __ctobpl_const_16: int;
+const {:extern} {:model_const "e->op1"} {:sourceFile ".\source\testex3.c"} {:sourceLine 16} unique __ctobpl_const_10: int;
 
 procedure {:extern} Eval(e.__1: int);
   free requires INT_LT(0, alloc);
-  modifies alloc, detChoiceCnt, Mem_T.INT4, Mem_T.op1__EXPR, Mem_T.op2__EXPR, Mem_T.oper__EXPR, Mem_T.result__EXPR;
   free ensures INT_LEQ(old(alloc), alloc);
-  free ensures Mem_T.INT4 == old(Mem_T.INT4);
-  free ensures Mem_T.op1__EXPR == old(Mem_T.op1__EXPR);
-  free ensures Mem_T.op2__EXPR == old(Mem_T.op2__EXPR);
-  free ensures Mem_T.oper__EXPR == old(Mem_T.oper__EXPR);
-  free ensures Mem_T.result__EXPR == old(Mem_T.result__EXPR);
 
 
 
@@ -562,54 +557,58 @@ implementation {:extern} Eval(e.__1: int)
   var {:extern} tempBoogie18: int;
   var {:extern} tempBoogie19: int;
 
-  anon0#2:
+  anon0:
     havoc_stringTemp := 0;
-    goto start#2;
+    goto start;
 
-  start#2:
+  start:
     assume INT_LT(e.__1, alloc);
     e := 0;
     e := e.__1;
-    goto label_3#2;
+    goto label_3;
 
-  label_3#2:
-    assert {:sourcefile "TestEx3.c"} {:sourceline 10} true;
+  label_3:
+    assert {:sourcefile ".\source\testex3.c"} {:sourceline 10} true;
     assert e != 0;
-    goto label_3_true#2, label_3_false#2;
+    goto label_3_true, label_3_false;
 
-  label_3_false#2:
+  label_3_false:
     assume !INT_EQ(Mem_T.oper__EXPR[oper__EXPR(e)], 1);
     assume value_is(__ctobpl_const_1, e);
     assume value_is(__ctobpl_const_2, Mem_T.oper__EXPR[oper__EXPR(e)]);
-    goto label_4#2;
+    goto label_4;
 
-  label_4#2:
-    assert {:sourcefile "TestEx3.c"} {:sourceline 14} true;
+  label_4:
+    assert {:sourcefile ".\source\testex3.c"} {:sourceline 14} true;
     assert e != 0;
-    goto label_4_true#2, label_4_false#2;
+    goto label_4_true, label_4_false;
 
-  label_4_false#2:
+  label_4_false:
     assume !INT_EQ(Mem_T.oper__EXPR[oper__EXPR(e)], 2);
     assume value_is(__ctobpl_const_3, e);
     assume value_is(__ctobpl_const_4, Mem_T.oper__EXPR[oper__EXPR(e)]);
-    goto label_6#2;
+    goto label_6;
 
-  label_6#2:
-    assert {:sourcefile "TestEx3.c"} {:sourceline 20} true;
+  label_6:
+    assert {:sourcefile ".\source\testex3.c"} {:sourceline 20} true;
     assert e != 0;
     Mem_T.result__EXPR := Mem_T.result__EXPR[result__EXPR(e) := -1];
     assume value_is(__ctobpl_const_5, e);
     assume value_is(__ctobpl_const_6, Mem_T.result__EXPR[result__EXPR(e)]);
-    goto label_1#2;
+    goto label_1;
 
-  label_4_true#2:
+  label_1:
+    assert {:sourcefile ".\source\testex3.c"} {:sourceline 22} true;
+    return;
+
+  label_4_true:
     assume INT_EQ(Mem_T.oper__EXPR[oper__EXPR(e)], 2);
     assume value_is(__ctobpl_const_3, e);
     assume value_is(__ctobpl_const_4, Mem_T.oper__EXPR[oper__EXPR(e)]);
-    goto label_7#2;
+    goto label_7;
 
-  label_7#2:
-    assert {:sourcefile "TestEx3.c"} {:sourceline 16} true;
+  label_7:
+    assert {:sourcefile ".\source\testex3.c"} {:sourceline 16} true;
     assert e != 0;
     assert e != 0;
     assert e != 0;
@@ -620,16 +619,16 @@ implementation {:extern} Eval(e.__1: int)
     assume value_is(__ctobpl_const_10, Mem_T.op1__EXPR[op1__EXPR(e)]);
     assume value_is(__ctobpl_const_11, e);
     assume value_is(__ctobpl_const_12, Mem_T.op2__EXPR[op2__EXPR(e)]);
-    goto label_1#2;
+    goto label_1;
 
-  label_3_true#2:
+  label_3_true:
     assume INT_EQ(Mem_T.oper__EXPR[oper__EXPR(e)], 1);
     assume value_is(__ctobpl_const_1, e);
     assume value_is(__ctobpl_const_2, Mem_T.oper__EXPR[oper__EXPR(e)]);
-    goto label_5#2;
+    goto label_5;
 
-  label_5#2:
-    assert {:sourcefile "TestEx3.c"} {:sourceline 12} true;
+  label_5:
+    assert {:sourcefile ".\source\testex3.c"} {:sourceline 12} true;
     assert e != 0;
     assert e != 0;
     assert e != 0;
@@ -640,11 +639,7 @@ implementation {:extern} Eval(e.__1: int)
     assume value_is(__ctobpl_const_16, Mem_T.op1__EXPR[op1__EXPR(e)]);
     assume value_is(__ctobpl_const_17, e);
     assume value_is(__ctobpl_const_18, Mem_T.op2__EXPR[op2__EXPR(e)]);
-    goto label_1#2;
-
-  label_1#2:
-    assert {:sourcefile "TestEx3.c"} {:sourceline 22} true;
-    return;
+    goto label_1;
 }
 
 
